\documentclass[12pt]{article}%
\usepackage{chicago}
\usepackage{graphicx}
\usepackage{amsmath}%
\setcounter{MaxMatrixCols}{30}%
\usepackage{amsfonts}%
\usepackage{amssymb}
%TCIDATA{OutputFilter=latex2.dll}
%TCIDATA{Version=5.50.0.2960}
%TCIDATA{CSTFile=article.cst}
%TCIDATA{Created=Wednesday, November 09, 2011 08:00:08}
%TCIDATA{LastRevised=Wednesday, November 09, 2011 08:16:38}
%TCIDATA{<META NAME="GraphicsSave" CONTENT="32">}
%TCIDATA{<META NAME="SaveForMode" CONTENT="1">}
%TCIDATA{BibliographyScheme=BibTeX}
%TCIDATA{<META NAME="DocumentShell" CONTENT="TTCA shells\TTCA-BriefReport">}
%BeginMSIPreambleData
\providecommand{\U}[1]{\protect\rule{.1in}{.1in}}
%EndMSIPreambleData
\begin{document}

\title{Title}
\author{Author}
\maketitle

\section{Converting the quartic equation for the ion Bohm velocity into a
fourth order polynomial}

Baalrud (55)%
\begin{equation}
\frac{n_{1}}{n_{e}}\frac{c_{s1}^{2}}{V_{1}^{2}}+\frac{n_{2}}{n_{e}}%
\frac{c_{s2}^{2}}{\left(  V_{1}-\Delta\right)  ^{2}}=1
\end{equation}
Multiply by $V_{1}^{2}$ and $\left(  V_{1}-\Delta V\right)  ^{2}$%
\begin{equation}
\frac{n_{1}}{n_{e}}c_{s1}^{2}\left(  V_{1}-\Delta\right)  ^{2}+\frac{n_{2}%
}{n_{e}}c_{s2}^{2}V_{1}^{2}=\left(  V_{1}-\Delta\right)  ^{2}V_{1}^{2}%
\end{equation}
Rearrange%
\begin{equation}
\left(  V_{1}-\Delta\right)  ^{2}V_{1}^{2}-\frac{n_{1}}{n_{e}}c_{s1}%
^{2}\left(  V_{1}-\Delta\right)  ^{2}-\frac{n_{2}}{n_{e}}c_{s2}^{2}V_{1}^{2}=0
\end{equation}
Expand%
\begin{equation}
\left(  V_{1}^{2}-2\Delta V_{1}+\Delta^{2}\right)  V_{1}^{2}-\frac{n_{1}%
}{n_{e}}c_{s1}^{2}\left(  V_{1}^{2}-2\Delta V_{1}+\Delta^{2}\right)
-\frac{n_{2}}{n_{e}}c_{s2}^{2}V_{1}^{2}=0
\end{equation}


Collect%
\begin{equation}
V_{1}^{4}-2\Delta V_{1}^{3}+\left(  \Delta^{2}-\frac{n_{1}}{n_{e}}c_{s1}%
^{2}-\frac{n_{2}}{n_{e}}c_{s2}^{2}\right)  V_{1}^{2}+2\Delta\frac{n_{1}}%
{n_{e}}c_{s1}^{2}V_{1}-\frac{n_{1}}{n_{e}}c_{s1}^{2}\Delta^{2}=0
\end{equation}
From the definition of the system sound speed%
\begin{equation}
c_{s}^{2}=\frac{n_{1}}{n_{e}}c_{s1}^{2}+\frac{n_{2}}{n_{e}}c_{s2}^{2}%
\end{equation}
we get%
\begin{equation}
V_{1}^{4}-2\Delta V_{1}^{3}+\left(  \Delta^{2}-c_{s}^{2}\right)  V_{1}%
^{2}+2\Delta\frac{n_{1}}{n_{e}}c_{s1}^{2}V_{1}-\frac{n_{1}}{n_{e}}c_{s1}%
^{2}\Delta^{2}=0
\end{equation}


\bibliographystyle{CHICAGO}
\bibliography{CommonAbbrevs,JournalNameAbbrevs}



\end{document}